did some work on Associativity

Fibonacci/Associativity.v
@@ -1,35 +1,129 @@
 Require Import List.
 Import ListNotations.
 
-Inductive Expr : Type :=
+Require Import Coq.Program.Wf.
+Require Import Lia.
+Require Import Coq.Arith.Arith.
+
+Definition Associative {A : Type} (op : A -> A -> A) : Prop :=
+  forall x y z : A, op x (op y z) = op (op x y) z.
+
+Inductive expr : Type :=
 | Num (n : nat)
-| Op (e1 e2 : Expr).
+| Op (e1 e2 : expr).
 
 Compute (Op (Num 1) (Num 2)).
 
-Fixpoint eval (e : Expr) (op : nat -> nat -> nat) : nat :=
+Fixpoint eval (op : nat -> nat -> nat) (e : expr) : nat :=
   match e with
   | Num n => n
-  | Op e1 e2 => op (eval e1 op) (eval e2 op)
+  | Op e1 e2 => op (eval op e1) (eval op e2)
   end.
 
-Definition e1 : Expr := Op (Num 1) (Num 2).
+Fixpoint elements (e : expr) : list nat :=
+  match e with
+  | Num n => [n]
+  | Op e1 e2 => elements e1 ++ elements e2
+  end.
 
-Compute (eval e1 mult).
+Definition e1 : expr := Op (Num 1) (Num 2).
+
+Compute (eval mult e1).
+
+Check (eval mult).
 
 Compute flat_map (fun n => map (fun m => m + n) ([1; 2; 3])) (seq 7 3).
 
-Fixpoint parenthesize (l : list nat) : list Expr :=
-  match l with
-  | [] => []
-  | x :: xs => match xs with
-                | [] => [Num x]
-                | _ :: _ =>
-                    flat_map
-                      (fun split_point : nat =>
-                      let left := firstn split_point l in
-                      let right := skipn split_point l in
-                      flat_map (fun el : Expr => map (fun er : Expr => Op el er) (parenthesize right)) (parenthesize left))
-                      (seq 1 (Nat.pred (length l)))
-                end
-  end.
+(* Define a well-founded relation based on the length of the list. *)
+Definition lengthOrder (l1 l2 : list nat) := length l1 < length l2.
+
+  Lemma lengthOrder_wf' : forall len, forall ls, length ls <= len -> Acc lengthOrder ls.
+    unfold lengthOrder. intros. induction ls.
+    - apply Acc_intro. intros. inversion H0.
+    - apply Acc_intro. intros. apply Acc_intro. intros. apply IHls.
+      -- simpl in H. lia.
+      -- assert (length y0 < length (a :: ls)) by lia. 
+         assert (length (a :: ls) = length ls + 1).
+         --- simpl. lia.
+         --- lia.
+  Defined.
+
+  Theorem lengthOrder_wf : well_founded lengthOrder.
+    red. intro. eapply lengthOrder_wf'. eauto.
+  Defined.
+  
+Lemma firstn_lengthOrder : forall (l : list nat) (n : nat),
+  n < length l -> lengthOrder (firstn n l) l.
+Proof.
+  intros l n. unfold lengthOrder. rewrite firstn_length. lia.
+Defined.
+
+Lemma skipn_lengthOrder : forall (l : list nat) (n : nat),
+  0 < n < length l -> lengthOrder (skipn n l) l.
+Proof.
+  intros l n. unfold lengthOrder. rewrite skipn_length. lia.
+Defined.
+
+Definition in_range (split_point len: nat) : {1 <= split_point <= Nat.pred len} + {split_point < 1 \/ Nat.pred len < split_point}.
+Proof.
+  destruct (le_lt_dec 1 split_point).
+  - destruct (le_lt_dec split_point (Nat.pred len)).
+    + left. lia.
+    + right. lia.
+  - right. lia.
+Defined.
+
+Definition parenthesize : list nat -> list expr.
+refine (Fix lengthOrder_wf (fun _ => list expr)
+  (fun (l : list nat)
+    (parenthesize : forall l' : list nat, lengthOrder l' l -> list expr) =>
+      match l with
+      | [] => []
+      | [x] => [Num x]  
+      | x :: xs => 
+        if le_lt_dec 2 (length l)
+        then     
+          flat_map
+            (fun split_point : nat =>
+              if in_range split_point (length l) then
+                let left := firstn split_point l in
+                let right := skipn split_point l in
+                flat_map (fun el : expr => map (fun er : expr => Op el er) (parenthesize right _)) (parenthesize left _)
+              else []
+            )
+            (seq 1 (Nat.pred (length l)))
+        else []
+      end)).
+  - apply skipn_lengthOrder. lia.
+  - apply firstn_lengthOrder. lia.
+Defined.
+
+Compute (last (parenthesize [1;2;3;4])).
+
+Compute (map (eval plus) (parenthesize [1;2;3;4;5;6;7;8])).
+
+Lemma lem2 : forall (l1 l2 : list nat) (op : nat -> nat -> nat), 
+  Associative op ->
+  fold_right op 0 (l1 ++ l2) = fold_right op 0 l1 + fold_right op 0 l2.
+Proof.
+  intros l1 l2. induction l1.
+  - intros op H. simpl. reflexivity.
+  - intros op H. simpl. rewrite IHl1.
+Qed.
+
+Check expr_ind.
+
+Lemma lem3 : forall (e : expr),
+  eval e = fold_right plus 0 (elements e).
+Proof.
+  intros e. induction e as [| e1 IH1 e2 IH2].
+  - simpl. lia.
+  - simpl. rewrite IH1. rewrite IH2. rewrite lem2. reflexivity.
+Qed.
+
+Theorem add_assoc_n : forall (e1 e2 : meaningful_expression),
+  elements e1 = elements e2 -> meaningful_sum e1 = meaningful_sum e2.
+Proof.
+  intros e1 e2 H.
+  repeat rewrite lem3. rewrite H. reflexivity.
+Qed.
